Prettified Semantics

pulse/ulib/experimental/Steel.Semantics.Hoare.MST.fst
@@ -27,7 +27,8 @@ open NMST
  * This module provides a semantic model for a combined effect of
  * divergence, state, and parallel composition of atomic actions.
  *
- * It is built over a monotonic state effect -- so that we can give lock semantics using monotonicity
+ * It is built over a monotonic state effect -- so that we can give
+ * lock semantics using monotonicity
  *
  * It also builds a generic separation-logic-style program logic
  * for this effect, in a partial correctness setting.
@@ -39,7 +40,6 @@ open NMST
  * these semantics.
  *
  * The program logic is specified in the Hoare-style pre- and postconditions
- *   See Steel.Semantics.fst for the wp variant
 *)
 
 
@@ -65,7 +65,7 @@ let transitive #a (equals:a -> a -> prop) =
   forall x y z. x `equals` y /\ y `equals` z ==> x `equals` z
 
 let associative #a (equals: a -> a -> prop) (f: a -> a -> a)=
-  forall x y z. //{:pattern f x (f y z) \/ f (f x y) z}
+  forall x y z.
     f x (f y z) `equals` f (f x y) z
 
 let commutative #a (equals: a -> a -> prop) (f: a -> a -> a) =
@@ -80,23 +80,32 @@ let is_unit #a (x:a) (equals: a -> a -> prop) (f:a -> a -> a) =
 let equals_ext #a (equals:a -> a -> prop) (f:a -> a -> a) =
   forall x1 x2 y. x1 `equals` x2 ==> f x1 y `equals` f x2 y
 
-let fp_heap_0 (#heap:Type) (#hprop:Type)
-              (interp:hprop -> heap -> prop)
-              (pre:hprop)
-    = h:heap{interp pre h}
+let fp_heap_0
+       (#heap:Type)
+       (#hprop:Type)
+       (interp:hprop -> heap -> prop)
+       (pre:hprop)
+    =
+  h:heap{interp pre h}
 
-let depends_only_on_0 (#heap:Type) (#hprop:Type)
-                      (interp:hprop -> heap -> prop)
-                      (disjoint: heap -> heap -> prop)
-                      (join: (h0:heap -> h1:heap{disjoint h0 h1} -> heap))
-                      (q:heap -> prop) (fp: hprop) =
-  (forall (h0:fp_heap_0 interp fp) (h1:heap{disjoint h0 h1}). q h0 <==> q (join h0 h1))
+let depends_only_on_0
+      (#heap:Type)
+      (#hprop:Type)
+      (interp:hprop -> heap -> prop)
+      (disjoint: heap -> heap -> prop)
+      (join: (h0:heap -> h1:heap{disjoint h0 h1} -> heap))
+      (q:heap -> prop) (fp: hprop)
+    =
+  forall (h0:fp_heap_0 interp fp) (h1:heap{disjoint h0 h1}). q h0 <==> q (join h0 h1)
 
-let fp_prop_0 (#heap:Type) (#hprop:Type)
-              (interp:hprop -> heap -> prop)
-              (disjoint: heap -> heap -> prop)
-              (join: (h0:heap -> h1:heap{disjoint h0 h1} -> heap))
-              (fp:hprop) =
+let fp_prop_0
+      (#heap:Type)
+      (#hprop:Type)
+      (interp:hprop -> heap -> prop)
+      (disjoint: heap -> heap -> prop)
+      (join: (h0:heap -> h1:heap{disjoint h0 h1} -> heap))
+      (fp:hprop)
+    =
   p:(heap -> prop){p `(depends_only_on_0 interp disjoint join)` fp}
 
 noeq
@@ -122,28 +131,28 @@ type st0 = {
 
 /// disjointness is symmetric
 
-let disjoint_sym (st:st0)
-  = forall h0 h1. st.disjoint h0 h1 <==> st.disjoint h1 h0
+let disjoint_sym (st:st0) =
+  forall h0 h1. st.disjoint h0 h1 <==> st.disjoint h1 h0
 
-let disjoint_join (st:st0)
-  = forall m0 m1 m2.
-       st.disjoint m1 m2 /\
-       st.disjoint m0 (st.join m1 m2) ==>
-       st.disjoint m0 m1 /\
-       st.disjoint m0 m2 /\
-       st.disjoint (st.join m0 m1) m2 /\
-       st.disjoint (st.join m0 m2) m1
+let disjoint_join (st:st0) =
+  forall m0 m1 m2.
+    st.disjoint m1 m2 /\
+    st.disjoint m0 (st.join m1 m2) ==>
+    st.disjoint m0 m1 /\
+    st.disjoint m0 m2 /\
+    st.disjoint (st.join m0 m1) m2 /\
+    st.disjoint (st.join m0 m2) m1
 
-let join_commutative (st:st0 { disjoint_sym st })
-  = forall m0 m1.
-      st.disjoint m0 m1 ==>
-      st.join m0 m1 == st.join m1 m0
+let join_commutative (st:st0 { disjoint_sym st }) =
+  forall m0 m1.
+    st.disjoint m0 m1 ==>
+    st.join m0 m1 == st.join m1 m0
 
-let join_associative (st:st0{disjoint_join st})
-  = forall m0 m1 m2.
-      st.disjoint m1 m2 /\
-      st.disjoint m0 (st.join m1 m2) ==>
-      st.join m0 (st.join m1 m2) == st.join (st.join m0 m1) m2
+let join_associative (st:st0{disjoint_join st})=
+  forall m0 m1 m2.
+    st.disjoint m1 m2 /\
+    st.disjoint m0 (st.join m1 m2) ==>
+    st.join m0 (st.join m1 m2) == st.join (st.join m0 m1) m2
 
 ////////////////////////////////////////////////////////////////////////////////
 
@@ -162,33 +171,33 @@ let depends_only_on (#st:st0) (q:st.mem -> prop) (fp: st.hprop) =
 let fp_prop (#st:st0) (fp:st.hprop) =
   fp_prop_0 st.interp st.disjoint st.join fp
 
-let lemma_weaken_depends_only_on (#st:st0{affine st})
-       (fp0 fp1:st.hprop)
-       (q:fp_prop fp0)
-  : Lemma (q `depends_only_on` (fp0 `st.star` fp1))
-  = ()
+let lemma_weaken_depends_only_on
+      (#st:st0{affine st})
+      (fp0 fp1:st.hprop)
+      (q:fp_prop fp0)
+    : Lemma (q `depends_only_on` (fp0 `st.star` fp1))
+    =
+  ()
 
 let st_laws (st:st0) =
-    (* standard laws about the equality relation *)
-    symmetry st.equals /\
-    transitive st.equals /\
-    interp_extensionality st.equals st.interp /\
-    (* standard laws for star forming a CM *)
-    associative st.equals st.star /\
-    commutative st.equals st.star /\
-    is_unit st.emp st.equals st.star /\
-    equals_ext st.equals st.star /\
-    (* We're working in an affine interpretation of SL *)
-    affine st /\
-    (* laws about disjoint and join *)
-    disjoint_sym st /\
-    disjoint_join st /\
-    join_commutative st /\
-    join_associative st
-
+  (* standard laws about the equality relation *)
+  symmetry st.equals /\
+  transitive st.equals /\
+  interp_extensionality st.equals st.interp /\
+  (* standard laws for star forming a CM *)
+  associative st.equals st.star /\
+  commutative st.equals st.star /\
+  is_unit st.emp st.equals st.star /\
+  equals_ext st.equals st.star /\
+  (* We're working in an affine interpretation of SL *)
+  affine st /\
+  (* laws about disjoint and join *)
+  disjoint_sym st /\
+  disjoint_join st /\
+  join_commutative st /\
+  join_associative st
 
 let st = s:st0 { st_laws s }
-
 
 (**** End state defn ****)
 
@@ -201,7 +210,6 @@ let st = s:st0 { st_laws s }
 /// provides, or the post heap assertion, is a st.hprop on [a]-typed result
 
 type post_t (st:st) (a:Type) = a -> st.hprop
-
 
 
 /// requires is a heap predicate that depends only on a pre heap assertion
@@ -222,44 +230,54 @@ let l_pre (#st:st) (pre:st.hprop) = fp_prop pre
 /// Also note that the support for depends_only_on_2 is not required from the underlying memory model
 
 
-let depends_only_on_0_2 (#a:Type) (#heap:Type) (#hprop:Type)
-  (interp:hprop -> heap -> prop)
-  (disjoint:heap -> heap -> prop)
-  (join:(h0:heap -> h1:heap{disjoint h0 h1} -> heap))
-  (q:heap -> a -> heap -> prop) (fp_pre:hprop) (fp_post:a -> hprop)
+let depends_only_on_0_2
+      (#a:Type)
+      (#heap:Type)
+      (#hprop:Type)
+      (interp:hprop -> heap -> prop)
+      (disjoint:heap -> heap -> prop)
+      (join:(h0:heap -> h1:heap{disjoint h0 h1} -> heap))
+      (q:heap -> a -> heap -> prop) (fp_pre:hprop) (fp_post:a -> hprop)
 
-= //can join any disjoint heap to the pre-heap and q is still valid
+    = //can join any disjoint heap to the pre-heap and q is still valid
   (forall x (h_pre:fp_heap_0 interp fp_pre) h_post (h:heap{disjoint h_pre h}).
      q h_pre x h_post <==> q (join h_pre h) x h_post) /\
-
   //can join any disjoint heap to the post-heap and q is still valid
   (forall x h_pre (h_post:fp_heap_0 interp (fp_post x)) (h:heap{disjoint h_post h}).
      q h_pre x h_post <==> q h_pre x (join h_post h))
 
-
 /// Abbreviations for two-state depends
 
-let fp_prop_0_2 (#a:Type) (#heap #hprop:Type)
-  (interp:hprop -> heap -> prop)
-  (disjoint:heap -> heap -> prop)
-  (join:(h0:heap -> h1:heap{disjoint h0 h1} -> heap))
-  (fp_pre:hprop) (fp_post:a -> hprop) =
-
+let fp_prop_0_2
+      (#a:Type)
+      (#heap #hprop:Type)
+      (interp:hprop -> heap -> prop)
+      (disjoint:heap -> heap -> prop)
+      (join:(h0:heap -> h1:heap{disjoint h0 h1} -> heap))
+      (fp_pre:hprop)
+      (fp_post:a -> hprop)
+    =
   q:(heap -> a -> heap -> prop){depends_only_on_0_2 interp disjoint join q fp_pre fp_post}
 
-let depends_only_on2 (#st:st0) (#a:Type) (q:st.mem -> a -> st.mem -> prop) (fp_pre:st.hprop) (fp_post:a -> st.hprop) =
+let depends_only_on2
+      (#st:st0)
+      (#a:Type)
+      (q:st.mem -> a -> st.mem -> prop)
+      (fp_pre:st.hprop)
+      (fp_post:a -> st.hprop)
+    =
   depends_only_on_0_2 st.interp st.disjoint st.join q fp_pre fp_post
 
 let fp_prop2 (#st:st0) (#a:Type) (fp_pre:st.hprop) (fp_post:a -> st.hprop) =
   q:(st.mem -> a -> st.mem -> prop){depends_only_on2 q fp_pre fp_post}
-
 
 /// Finally the type of 2-state postconditions
 
 let l_post (#st:st) (#a:Type) (pre:st.hprop) (post:post_t st a) = fp_prop2 pre post
 
 
-(**** End expects, provides, requires, and ensures defns ****)
+(**** End expects, provides, requires,
+      and ensures defns ****)
 
 effect Mst (a:Type) (#st:st) (req:st.mem -> Type0) (ens:st.mem -> a -> st.mem -> Type0) =
   NMSTATE a st.mem st.locks_preorder req ens
@@ -275,16 +293,23 @@ let preserves_frame (#st:st) (pre post:st.hprop) (m0 m1:st.mem) =
     (st.interp ((post `st.star` frame) `st.star` (st.locks_invariant m1)) m1 /\
      (forall (f_frame:fp_prop frame). f_frame (st.core m0) == f_frame (st.core m1)))
 
-let action_t (#st:st) (#a:Type) (pre:st.hprop) (post:post_t st a) (lpre:l_pre pre) (lpost:l_post pre post) =
+let action_t
+      (#st:st)
+      (#a:Type)
+      (pre:st.hprop)
+      (post:post_t st a)
+      (lpre:l_pre pre)
+      (lpost:l_post pre post)
+    =
   unit ->
-  Mst a
-  (requires fun m0 ->
-    st.interp (pre `st.star` st.locks_invariant m0) m0 /\
-    lpre (st.core m0))
-  (ensures fun m0 x m1 ->
-    st.interp ((post x) `st.star` st.locks_invariant m1) m1 /\
-    lpost (st.core m0) x (st.core m1) /\
-    preserves_frame pre (post x) m0 m1)
+    Mst a
+      (requires fun m0 ->
+        st.interp (pre `st.star` st.locks_invariant m0) m0 /\
+        lpre (st.core m0))
+      (ensures fun m0 x m1 ->
+        st.interp ((post x) `st.star` st.locks_invariant m1) m1 /\
+        lpost (st.core m0) x (st.core m1) /\
+        preserves_frame pre (post x) m0 m1)
 
 (**** End interface of actions ****)
 
@@ -298,66 +323,107 @@ let action_t (#st:st) (#a:Type) (pre:st.hprop) (post:post_t st a) (lpre:l_pre pr
 /// Return node is parametric in provides and ensures
 
 let return_lpre (#st:st) (#a:Type) (#post:post_t st a) (x:a) (lpost:l_post (post x) post)
-: l_pre (post x)
-= fun h -> lpost h x h
+    : l_pre (post x)
+    =
+  fun h -> lpost h x h
 
 let frame_lpre (#st:st) (#pre:st.hprop) (lpre:l_pre pre) (#frame:st.hprop) (f_frame:fp_prop frame)
-: l_pre (pre `st.star` frame)
-= fun h -> lpre h /\ f_frame h
+    : l_pre (pre `st.star` frame)
+    =
+  fun h -> lpre h /\ f_frame h
 
-let frame_lpost (#st:st) (#a:Type) (#pre:st.hprop) (#post:post_t st a) (lpre:l_pre pre) (lpost:l_post pre post)
-  (#frame:st.hprop) (f_frame:fp_prop frame)
-: l_post (pre `st.star` frame) (fun x -> post x `st.star` frame)
-= fun h0 x h1 -> lpre h0 /\ lpost h0 x h1 /\ f_frame h1
-
+let frame_lpost
+      (#st:st)
+      (#a:Type)
+      (#pre:st.hprop)
+      (#post:post_t st a)
+      (lpre:l_pre pre)
+      (lpost:l_post pre post)
+      (#frame:st.hprop)
+      (f_frame:fp_prop frame)
+    : l_post (pre `st.star` frame) (fun x -> post x `st.star` frame)
+    =
+  fun h0 x h1 -> lpre h0 /\ lpost h0 x h1 /\ f_frame h1
 
 /// The bind rule bakes in weakening of requires / ensures
 
-let bind_lpre (#st:st) (#a:Type) (#pre:st.hprop) (#post_a:post_t st a)
-  (lpre_a:l_pre pre) (lpost_a:l_post pre post_a)
-  (lpre_b:(x:a -> l_pre (post_a x)))
-: l_pre pre
-= fun h -> lpre_a h /\ (forall (x:a) h1. lpost_a h x h1 ==> lpre_b x h1)
+let bind_lpre
+      (#st:st)
+      (#a:Type)
+      (#pre:st.hprop)
+      (#post_a:post_t st a)
+      (lpre_a:l_pre pre)
+      (lpost_a:l_post pre post_a)
+      (lpre_b:(x:a -> l_pre (post_a x)))
+    : l_pre pre
+    =
+  fun h -> lpre_a h /\ (forall (x:a) h1. lpost_a h x h1 ==> lpre_b x h1)
 
-let bind_lpost (#st:st) (#a:Type) (#pre:st.hprop) (#post_a:post_t st a)
-  (lpre_a:l_pre pre) (lpost_a:l_post pre post_a)
-  (#b:Type) (#post_b:post_t st b)
-  (lpost_b:(x:a -> l_post (post_a x) post_b))
-: l_post pre post_b
-= fun h0 y h2 -> lpre_a h0 /\ (exists x h1. lpost_a h0 x h1 /\ (lpost_b x) h1 y h2)
-
+let bind_lpost
+      (#st:st)
+      (#a:Type)
+      (#pre:st.hprop)
+      (#post_a:post_t st a)
+      (lpre_a:l_pre pre)
+      (lpost_a:l_post pre post_a)
+      (#b:Type)
+      (#post_b:post_t st b)
+      (lpost_b:(x:a -> l_post (post_a x) post_b))
+    : l_post pre post_b
+    =
+  fun h0 y h2 -> lpre_a h0 /\ (exists x h1. lpost_a h0 x h1 /\ (lpost_b x) h1 y h2)
 
 /// Parallel composition is pointwise
 
-let par_lpre (#st:st) (#preL:st.hprop) (lpreL:l_pre preL)
-  (#preR:st.hprop) (lpreR:l_pre preR)
-: l_pre (preL `st.star` preR)
-= fun h -> lpreL h /\ lpreR h
+let par_lpre
+       (#st:st)
+       (#preL:st.hprop)
+       (lpreL:l_pre preL)
+       (#preR:st.hprop)
+       (lpreR:l_pre preR)
+    : l_pre (preL `st.star` preR)
+    =
+  fun h -> lpreL h /\ lpreR h
 
-let par_lpost (#st:st) (#aL:Type) (#preL:st.hprop) (#postL:post_t st aL)
-  (lpreL:l_pre preL) (lpostL:l_post preL postL)
-  (#aR:Type) (#preR:st.hprop) (#postR:post_t st aR)
-  (lpreR:l_pre preR) (lpostR:l_post preR postR)
-: l_post (preL `st.star` preR) (fun (xL, xR) -> postL xL `st.star` postR xR)
-= fun h0 (xL, xR) h1 -> lpreL h0 /\ lpreR h0 /\ lpostL h0 xL h1 /\ lpostR h0 xR h1
+let par_lpost
+      (#st:st)
+      (#aL:Type)
+      (#preL:st.hprop)
+      (#postL:post_t st aL)
+      (lpreL:l_pre preL)
+      (lpostL:l_post preL postL)
+      (#aR:Type)
+      (#preR:st.hprop)
+      (#postR:post_t st aR)
+      (lpreR:l_pre preR)
+      (lpostR:l_post preR postR)
+    : l_post (preL `st.star` preR) (fun (xL, xR) -> postL xL `st.star` postR xR)
+    =
+  fun h0 (xL, xR) h1 -> lpreL h0 /\ lpreR h0 /\ lpostL h0 xL h1 /\ lpostR h0 xR h1
 
-let weaker_pre (#st:st)
-  (pre:st.hprop) (next_pre:st.hprop)
-= forall (h:st.mem) (frame:st.hprop).
+let weaker_pre (#st:st) (pre:st.hprop) (next_pre:st.hprop) =
+  forall (h:st.mem) (frame:st.hprop).
     st.interp (pre `st.star` frame) h ==>
     st.interp (next_pre `st.star` frame) h
 
-let stronger_post (#st:st) (#a:Type u#a)
-  (post next_post:post_t st a)
-= forall (x:a) (h:st.mem) (frame:st.hprop).
+let stronger_post (#st:st) (#a:Type u#a) (post next_post:post_t st a) =
+  forall (x:a) (h:st.mem) (frame:st.hprop).
     st.interp (next_post x `st.star` frame) h ==>
     st.interp (post x `st.star` frame) h
 
-
-let weakening_ok (#st:st) (#a:Type u#a)
-  (#pre:st.hprop) (#post:post_t st a) (lpre:l_pre pre) (lpost:l_post pre post)
-  (#wpre:st.hprop) (#wpost:post_t st a) (wlpre:l_pre wpre) (wlpost:l_post wpre wpost)
-= weaker_pre wpre pre /\
+let weakening_ok
+      (#st:st)
+      (#a:Type u#a)
+      (#pre:st.hprop)
+      (#post:post_t st a)
+      (lpre:l_pre pre)
+      (lpost:l_post pre post)
+      (#wpre:st.hprop)
+      (#wpost:post_t st a)
+      (wlpre:l_pre wpre)
+      (wlpost:l_post wpre wpost)
+    =
+  weaker_pre wpre pre /\
   stronger_post wpost post /\
   (forall h. wlpre h ==> lpre h) /\
   (forall h0 x h1. lpost h0 x h1 ==> wlpost h0 x h1)
@@ -367,7 +433,13 @@ let weakening_ok (#st:st) (#a:Type u#a)
 
 #push-options "--__temp_no_proj Steel.Semantics.Hoare.MST"
 noeq
-type m (st:st) : a:Type u#a -> pre:st.hprop -> post:post_t st a -> l_pre pre -> l_post pre post -> Type =
+type m (st:st) :
+      a:Type u#a ->
+      pre:st.hprop ->
+      post:post_t st a ->
+      l_pre pre ->
+      l_post pre post -> Type
+    =
   | Ret:
     #a:Type u#a ->
     post:post_t st a ->
@@ -482,42 +554,64 @@ type step_result (st:st) (a:Type u#a) =
 
 
 unfold
-let step_req (#st:st)
-  (#a:Type u#a) (#pre:st.hprop) (#post:post_t st a) (#lpre:l_pre pre) (#lpost:l_post pre post)
-  (f:m st a pre post lpre lpost)
-: st.mem -> Type0
-= fun m0 ->
-  st.interp (pre `st.star` st.locks_invariant m0) m0 /\
-  lpre (st.core m0)
+let step_req
+      (#st:st)
+      (#a:Type u#a)
+      (#pre:st.hprop)
+      (#post:post_t st a)
+      (#lpre:l_pre pre)
+      (#lpost:l_post pre post)
+      (f:m st a pre post lpre lpost)
+    : st.mem -> Type0
+    =
+  fun m0 ->
+    st.interp (pre `st.star` st.locks_invariant m0) m0 /\
+    lpre (st.core m0)
 
-let weaker_lpre (#st:st)
-  (#pre:st.hprop) (lpre:l_pre pre)
-  (#next_pre:st.hprop) (next_lpre:l_pre next_pre)
-  (m0 m1:st.mem)
-= lpre (st.core m0) ==> next_lpre (st.core m1)
+let weaker_lpre
+      (#st:st)
+      (#pre:st.hprop)
+      (lpre:l_pre pre)
+      (#next_pre:st.hprop)
+      (next_lpre:l_pre next_pre)
+      (m0 m1:st.mem)
+    =
+  lpre (st.core m0) ==> next_lpre (st.core m1)
 
-let stronger_lpost (#st:st) (#a:Type u#a)
-  (#pre:st.hprop) (#post:post_t st a)
-  (lpost:l_post pre post)
-  (#next_pre:st.hprop) #next_post (next_lpost:l_post next_pre next_post)
-  (m0 m1:st.mem)
-= forall (x:a) (h_final:st.mem).
+let stronger_lpost
+      (#st:st)
+      (#a:Type u#a)
+      (#pre:st.hprop)
+      (#post:post_t st a)
+      (lpost:l_post pre post)
+      (#next_pre:st.hprop)
+      #next_post
+      (next_lpost:l_post next_pre next_post)
+      (m0 m1:st.mem)
+    =
+  forall (x:a) (h_final:st.mem).
     next_lpost (st.core m1) x h_final ==>
     lpost (st.core m0) x h_final
 
 unfold
-let step_ens (#st:st)
-  (#a:Type u#a) (#pre:st.hprop) (#post:post_t st a) (#lpre:l_pre pre) (#lpost:l_post pre post)
-  (f:m st a pre post lpre lpost)
-: st.mem -> step_result st a -> st.mem -> Type0
-= fun m0 r m1 ->
-  let Step next_pre next_post next_lpre next_lpost _ = r in
-  st.interp (next_pre `st.star` st.locks_invariant m1) m1 /\
-  stronger_post post next_post /\
-  next_lpre (st.core m1) /\
-  preserves_frame pre next_pre m0 m1 /\
-  weaker_lpre lpre next_lpre m0 m1 /\
-  stronger_lpost lpost next_lpost m0 m1
+let step_ens
+      (#st:st)
+      (#a:Type u#a)
+      (#pre:st.hprop)
+      (#post:post_t st a)
+      (#lpre:l_pre pre)
+      (#lpost:l_post pre post)
+      (f:m st a pre post lpre lpost)
+    : st.mem -> step_result st a -> st.mem -> Type0
+    =
+  fun m0 r m1 ->
+    let Step next_pre next_post next_lpre next_lpost _ = r in
+    st.interp (next_pre `st.star` st.locks_invariant m1) m1 /\
+    stronger_post post next_post /\
+    next_lpre (st.core m1) /\
+    preserves_frame pre next_pre m0 m1 /\
+    weaker_lpre lpre next_lpre m0 m1 /\
+    stronger_lpost lpost next_lpost m0 m1
 
 
 /// The type of the stepping function
@@ -525,7 +619,10 @@ let step_ens (#st:st)
 type step_t =
   #st:st ->
   #a:Type u#a ->
-  #pre:st.hprop -> #post:post_t st a -> #lpre:l_pre pre -> #lpost:l_post pre post ->
+  #pre:st.hprop ->
+  #post:post_t st a ->
+  #lpre:l_pre pre ->
+  #lpost:l_post pre post ->
   f:m st a pre post lpre lpost ->
   Mst (step_result st a) (step_req f) (step_ens f)
 
@@ -535,20 +632,23 @@ type step_t =
 /// Some AC lemmas on `st.star`
 
 let apply_assoc (#st:st) (p q r:st.hprop)
-: Lemma (st.equals (p `st.star` (q `st.star` r)) ((p `st.star` q) `st.star` r))
-= ()
+    : Lemma (st.equals (p `st.star` (q `st.star` r)) ((p `st.star` q) `st.star` r))
+    =
+  ()
 
 let equals_ext_left (#st:st) (p q r:st.hprop)
-: Lemma
-  (requires p `st.equals` q)
-  (ensures (p `st.star` r) `st.equals` (q `st.star` r))
-= ()
+    : Lemma
+      (requires p `st.equals` q)
+      (ensures (p `st.star` r) `st.equals` (q `st.star` r))
+    =
+  ()
 
 let equals_ext_right (#st:st) (p q r:st.hprop)
-: Lemma
-  (requires q `st.equals` r)
-  (ensures (p `st.star` q) `st.equals` (p `st.star` r))
-= calc (st.equals) {
+    : Lemma
+      (requires q `st.equals` r)
+      (ensures (p `st.star` q) `st.equals` (p `st.star` r))
+    =
+  calc (st.equals) {
     p `st.star` q;
        (st.equals) { }
     q `st.star` p;
@@ -559,20 +659,22 @@ let equals_ext_right (#st:st) (p q r:st.hprop)
   }
 
 let commute_star_right (#st:st) (p q r:st.hprop)
-: Lemma
-  ((p `st.star` (q `st.star` r)) `st.equals`
-   (p `st.star` (r `st.star` q)))
-= calc (st.equals) {
+    : Lemma
+      ((p `st.star` (q `st.star` r)) `st.equals`
+        (p `st.star` (r `st.star` q)))
+    =
+  calc (st.equals) {
     p `st.star` (q `st.star` r);
        (st.equals) { equals_ext_right p (q `st.star` r) (r `st.star` q) }
     p `st.star` (r `st.star` q);
   }
 
 let assoc_star_right (#st:st) (p q r s:st.hprop)
-: Lemma
-  ((p `st.star` ((q `st.star` r) `st.star` s)) `st.equals`
-   (p `st.star` (q `st.star` (r `st.star` s))))
-= calc (st.equals) {
+    : Lemma
+      ((p `st.star` ((q `st.star` r) `st.star` s)) `st.equals`
+        (p `st.star` (q `st.star` (r `st.star` s))))
+    =
+  calc (st.equals) {
     p `st.star` ((q `st.star` r) `st.star` s);
        (st.equals) { equals_ext_right p ((q `st.star` r) `st.star` s)
                                         (q `st.star` (r `st.star` s)) }
@@ -580,10 +682,11 @@ let assoc_star_right (#st:st) (p q r s:st.hprop)
   }
 
 let commute_assoc_star_right (#st:st) (p q r s:st.hprop)
-: Lemma
-  ((p `st.star` ((q `st.star` r) `st.star` s)) `st.equals`
-   (p `st.star` (r `st.star` (q `st.star` s))))
-= calc (st.equals) {
+    : Lemma
+      ((p `st.star` ((q `st.star` r) `st.star` s)) `st.equals`
+        (p `st.star` (r `st.star` (q `st.star` s))))
+    =
+  calc (st.equals) {
     p `st.star` ((q `st.star` r) `st.star` s);
        (st.equals) { equals_ext_right p
                        ((q `st.star` r) `st.star` s)
@@ -597,148 +700,161 @@ let commute_assoc_star_right (#st:st) (p q r s:st.hprop)
 /// Apply extensionality manually, control proofs
 
 let apply_interp_ext (#st:st) (p q:st.hprop) (m:st.mem)
-: Lemma
-  (requires
-    st.interp p m /\
-    p `st.equals` q)
-  (ensures st.interp q m)
-= ()
+    : Lemma
+      (requires (st.interp p m /\ p `st.equals` q))
+      (ensures st.interp q m)
+    =
+  ()
 
 let weaken_fp_prop (#st:st) (frame frame':st.hprop) (m0 m1:st.mem)
-: Lemma
-  (requires
-    forall (f_frame:fp_prop (frame `st.star` frame')).
-      f_frame (st.core m0) ==
-      f_frame (st.core m1))
-   (ensures
-    forall (f_frame:fp_prop frame').
-      f_frame (st.core m0) ==
-      f_frame (st.core m1))
-= ()
+    : Lemma
+      (requires
+        forall (f_frame:fp_prop (frame `st.star` frame')).
+          f_frame (st.core m0) == f_frame (st.core m1))
+     (ensures
+       forall (f_frame:fp_prop frame').
+         f_frame (st.core m0) == f_frame (st.core m1))
+    =
+  ()
 
-let depends_only_on_commutes_with_weaker (#st:st) (q:st.mem -> prop) (fp:st.hprop) (fp_next:st.hprop)
-: Lemma
-  (requires
-    depends_only_on q fp /\
-    weaker_pre fp_next fp)
-  (ensures depends_only_on q fp_next)
-= assert (forall (h0:fp_heap_0 st.interp fp_next). st.interp (fp_next `st.star` st.emp) h0)
+let depends_only_on_commutes_with_weaker
+      (#st:st)
+      (q:st.mem -> prop)
+      (fp:st.hprop)
+      (fp_next:st.hprop)
+    : Lemma
+      (requires depends_only_on q fp /\ weaker_pre fp_next fp)
+      (ensures depends_only_on q fp_next)
+    =
+  assert (forall (h0:fp_heap_0 st.interp fp_next). st.interp (fp_next `st.star` st.emp) h0)
 
-let depends_only_on2_commutes_with_weaker (#st:st) (#a:Type)
-  (q:st.mem -> a -> st.mem -> prop) (fp:st.hprop) (fp_next:st.hprop) (fp_post:a -> st.hprop)
-: Lemma
-  (requires
-    depends_only_on2 q fp fp_post /\
-    weaker_pre fp_next fp)
-  (ensures depends_only_on2 q fp_next fp_post)
-= assert (forall (h0:fp_heap_0 st.interp fp_next). st.interp (fp_next `st.star` st.emp) h0)
+let depends_only_on2_commutes_with_weaker
+      (#st:st)
+      (#a:Type)
+      (q:st.mem -> a -> st.mem -> prop)
+      (fp:st.hprop)
+      (fp_next:st.hprop)
+      (fp_post:a -> st.hprop)
+    : Lemma
+      (requires depends_only_on2 q fp fp_post /\ weaker_pre fp_next fp)
+      (ensures depends_only_on2 q fp_next fp_post)
+    =
+  assert (forall (h0:fp_heap_0 st.interp fp_next). st.interp (fp_next `st.star` st.emp) h0)
 
 /// Lemmas about preserves_frame
 
-let preserves_frame_trans (#st:st)
-  (hp1 hp2 hp3:st.hprop) (m1 m2 m3:st.mem)
-: Lemma
-  (requires
-    preserves_frame hp1 hp2 m1 m2 /\
-    preserves_frame hp2 hp3 m2 m3)
-  (ensures preserves_frame hp1 hp3 m1 m3)
-= ()
+let preserves_frame_trans
+      (#st:st)
+      (hp1 hp2 hp3:st.hprop)
+      (m1 m2 m3:st.mem)
+    : Lemma
+      (requires preserves_frame hp1 hp2 m1 m2 /\ preserves_frame hp2 hp3 m2 m3)
+      (ensures preserves_frame hp1 hp3 m1 m3)
+    =
+  ()
 
 #push-options "--warn_error -271"
-let preserves_frame_stronger_post (#st:st) (#a:Type)
-  (pre:st.hprop) (post post_s:post_t st a) (x:a) (m1 m2:st.mem)
-: Lemma
-  (requires
-    preserves_frame pre (post_s x) m1 m2 /\
-    stronger_post post post_s)
-  (ensures preserves_frame pre (post x) m1 m2)
-= let aux (frame:st.hprop)
+let preserves_frame_stronger_post
+      (#st:st)
+      (#a:Type)
+      (pre:st.hprop)
+      (post post_s:post_t st a)
+      (x:a)
+      (m1 m2:st.mem)
     : Lemma
-      (requires st.interp (st.locks_invariant m1 `st.star` (pre `st.star` frame)) m1)
-      (ensures
-        st.interp (st.locks_invariant m2 `st.star` (post x `st.star` frame)) m2 /\
-        (forall (f_frame:fp_prop frame). f_frame (st.core m1) == f_frame (st.core m2)))
-      [SMTPat ()]
-    = assert (st.interp (st.locks_invariant m2 `st.star` (post_s x `st.star` frame)) m2);
-
-      calc (st.equals) {
-        st.locks_invariant m2 `st.star` (post_s x `st.star` frame);
-           (st.equals) { }
-        (st.locks_invariant m2 `st.star` post_s x) `st.star` frame;
-           (st.equals) { }
-        (post_s x `st.star` st.locks_invariant m2) `st.star` frame;
-           (st.equals) { }
-        post_s x `st.star` (st.locks_invariant m2 `st.star` frame);
+      (requires preserves_frame pre (post_s x) m1 m2 /\ stronger_post post post_s)
+      (ensures preserves_frame pre (post x) m1 m2)
+    =
+  let aux (frame:st.hprop)
+      : Lemma
+        (requires st.interp (st.locks_invariant m1 `st.star` (pre `st.star` frame)) m1)
+        (ensures
+          st.interp (st.locks_invariant m2 `st.star` (post x `st.star` frame)) m2 /\
+          (forall (f_frame:fp_prop frame). f_frame (st.core m1) == f_frame (st.core m2)))
+        [SMTPat ()]
+      =
+    assert (st.interp (st.locks_invariant m2 `st.star` (post_s x `st.star` frame)) m2);
+    calc (st.equals) {
+      st.locks_invariant m2 `st.star` (post_s x `st.star` frame);
+         (st.equals) { }
+      (st.locks_invariant m2 `st.star` post_s x) `st.star` frame;
+         (st.equals) { }
+      (post_s x `st.star` st.locks_invariant m2) `st.star` frame;
+         (st.equals) { }
+     post_s x `st.star` (st.locks_invariant m2 `st.star` frame);
+    };
+    assert (st.interp (post_s x `st.star` (st.locks_invariant m2 `st.star` frame)) m2);
+    assert (st.interp (post x `st.star` (st.locks_invariant m2 `st.star` frame)) m2);
+    calc (st.equals) {
+      post x `st.star` (st.locks_invariant m2 `st.star` frame);
+         (st.equals) { }
+      (post x `st.star` st.locks_invariant m2) `st.star` frame;
+         (st.equals) { }
+      (st.locks_invariant m2 `st.star` post x) `st.star` frame;
+         (st.equals) { apply_assoc (st.locks_invariant m2) (post x) frame }
+      st.locks_invariant m2 `st.star` (post x `st.star` frame);
       };
-
-      assert (st.interp (post_s x `st.star` (st.locks_invariant m2 `st.star` frame)) m2);
-      assert (st.interp (post x `st.star` (st.locks_invariant m2 `st.star` frame)) m2);
-
-      calc (st.equals) {
-        post x `st.star` (st.locks_invariant m2 `st.star` frame);
-           (st.equals) { }
-        (post x `st.star` st.locks_invariant m2) `st.star` frame;
-           (st.equals) { }
-        (st.locks_invariant m2 `st.star` post x) `st.star` frame;
-           (st.equals) { apply_assoc (st.locks_invariant m2) (post x) frame }
-        st.locks_invariant m2 `st.star` (post x `st.star` frame);
-      };
-
-      assert (st.interp (st.locks_invariant m2 `st.star` (post x `st.star` frame)) m2)
+    assert (st.interp (st.locks_invariant m2 `st.star` (post x `st.star` frame)) m2)
   in
   ()
 #pop-options
 
 #push-options "--z3rlimit 40 --warn_error -271"
 let preserves_frame_star (#st:st) (pre post:st.hprop) (m0 m1:st.mem) (frame:st.hprop)
-: Lemma
-  (requires preserves_frame pre post m0 m1)
-  (ensures preserves_frame (pre `st.star` frame) (post `st.star` frame) m0 m1)
-= let aux (frame':st.hprop)
     : Lemma
-      (requires
-        st.interp (st.locks_invariant m0 `st.star` ((pre `st.star` frame) `st.star` frame')) m0)
-      (ensures
-        st.interp (st.locks_invariant m1 `st.star` ((post `st.star` frame) `st.star` frame')) m1 /\
-        (forall (f_frame:fp_prop frame'). f_frame (st.core m0) == f_frame (st.core m1)))
-      [SMTPat ()]
-    = assoc_star_right (st.locks_invariant m0) pre frame frame';
-      apply_interp_ext
-        (st.locks_invariant m0 `st.star` ((pre `st.star` frame) `st.star` frame'))
-        (st.locks_invariant m0 `st.star` (pre `st.star` (frame `st.star` frame')))
-        m0;
-      assoc_star_right (st.locks_invariant m1) post frame frame';
-      apply_interp_ext
-        (st.locks_invariant m1 `st.star` (post `st.star` (frame `st.star` frame')))
-        (st.locks_invariant m1 `st.star` ((post `st.star` frame) `st.star` frame'))
-        m1;
-      weaken_fp_prop frame frame' m0 m1
+      (requires preserves_frame pre post m0 m1)
+      (ensures preserves_frame (pre `st.star` frame) (post `st.star` frame) m0 m1)
+    =
+  let aux (frame':st.hprop)
+      : Lemma
+        (requires
+          st.interp (st.locks_invariant m0 `st.star` ((pre `st.star` frame) `st.star` frame')) m0)
+        (ensures
+          st.interp (st.locks_invariant m1 `st.star`
+            ((post `st.star` frame) `st.star` frame')) m1 /\
+          (forall (f_frame:fp_prop frame'). f_frame (st.core m0) == f_frame (st.core m1)))
+        [SMTPat ()]
+      =
+    assoc_star_right (st.locks_invariant m0) pre frame frame';
+    apply_interp_ext
+      (st.locks_invariant m0 `st.star` ((pre `st.star` frame) `st.star` frame'))
+      (st.locks_invariant m0 `st.star` (pre `st.star` (frame `st.star` frame')))
+      m0;
+    assoc_star_right (st.locks_invariant m1) post frame frame';
+    apply_interp_ext
+      (st.locks_invariant m1 `st.star` (post `st.star` (frame `st.star` frame')))
+      (st.locks_invariant m1 `st.star` ((post `st.star` frame) `st.star` frame'))
+      m1;
+    weaken_fp_prop frame frame' m0 m1
   in
   ()
 
 let preserves_frame_star_left (#st:st) (pre post:st.hprop) (m0 m1:st.mem) (frame:st.hprop)
-: Lemma
-  (requires preserves_frame pre post m0 m1)
-  (ensures preserves_frame (frame `st.star` pre) (frame `st.star` post) m0 m1)
-= let aux (frame':st.hprop)
     : Lemma
-      (requires
-        st.interp (st.locks_invariant m0 `st.star` ((frame `st.star` pre) `st.star` frame')) m0)
-      (ensures
-        st.interp (st.locks_invariant m1 `st.star` ((frame `st.star` post) `st.star` frame')) m1 /\
-        (forall (f_frame:fp_prop frame'). f_frame (st.core m0) == f_frame (st.core m1)))
-      [SMTPat ()]
-    = commute_assoc_star_right (st.locks_invariant m0) frame pre frame';
-      apply_interp_ext
-        (st.locks_invariant m0 `st.star` ((frame `st.star` pre) `st.star` frame'))
-        (st.locks_invariant m0 `st.star` (pre `st.star` (frame `st.star` frame')))
-        m0;
-      commute_assoc_star_right (st.locks_invariant m1) frame post frame';
-      apply_interp_ext
-        (st.locks_invariant m1 `st.star` (post `st.star` (frame `st.star` frame')))
-        (st.locks_invariant m1 `st.star` ((frame `st.star` post) `st.star` frame'))
-        m1;
-      weaken_fp_prop frame frame' m0 m1
+      (requires preserves_frame pre post m0 m1)
+      (ensures preserves_frame (frame `st.star` pre) (frame `st.star` post) m0 m1)
+    =
+  let aux (frame':st.hprop)
+      : Lemma
+        (requires
+          st.interp (st.locks_invariant m0 `st.star` ((frame `st.star` pre) `st.star` frame')) m0)
+        (ensures
+          st.interp (st.locks_invariant m1 `st.star`
+            ((frame `st.star` post) `st.star` frame')) m1 /\
+          (forall (f_frame:fp_prop frame'). f_frame (st.core m0) == f_frame (st.core m1)))
+        [SMTPat ()]
+      =
+    commute_assoc_star_right (st.locks_invariant m0) frame pre frame';
+    apply_interp_ext
+      (st.locks_invariant m0 `st.star` ((frame `st.star` pre) `st.star` frame'))
+      (st.locks_invariant m0 `st.star` (pre `st.star` (frame `st.star` frame')))
+      m0;
+    commute_assoc_star_right (st.locks_invariant m1) frame post frame';
+    apply_interp_ext
+      (st.locks_invariant m1 `st.star` (post `st.star` (frame `st.star` frame')))
+      (st.locks_invariant m1 `st.star` ((frame `st.star` post) `st.star` frame'))
+      m1;
+    weaken_fp_prop frame frame' m0 m1
   in
   ()
 #pop-options
@@ -761,104 +877,146 @@ let preserves_frame_star_left (#st:st) (pre post:st.hprop) (m0 m1:st.mem) (frame
 ///
 /// To use it, we instantiate the fp prop with inst_heap_prop_for_par
 
-let inst_heap_prop_for_par (#st:st) (#a:Type) (#pre:st.hprop) (#post:post_t st a)
-  (lpost:l_post pre post)
-  (state:st.mem)
-: fp_prop pre
-= fun h ->
-  forall x final_state. lpost h x final_state <==>
-                   lpost (st.core state) x final_state
+let inst_heap_prop_for_par
+      (#st:st)
+      (#a:Type)
+      (#pre:st.hprop)
+      (#post:post_t st a)
+      (lpost:l_post pre post)
+      (state:st.mem)
+    : fp_prop pre
+    =
+  fun h ->
+    forall x final_state.
+      lpost h x final_state <==>
+      lpost (st.core state) x final_state
 
-let frame_post_for_par_tautology (#st:st)
-  (#a:Type) (#pre_f:st.hprop) (#post_f:post_t st a) (lpost_f:l_post pre_f post_f)
-  (m0:st.mem)
-: Lemma (inst_heap_prop_for_par lpost_f m0 (st.core m0))
-= ()
+let frame_post_for_par_tautology
+      (#st:st)
+      (#a:Type)
+      (#pre_f:st.hprop)
+      (#post_f:post_t st a)
+      (lpost_f:l_post pre_f post_f)
+      (m0:st.mem)
+    : Lemma (inst_heap_prop_for_par lpost_f m0 (st.core m0))
+    =
+  ()
 
-let frame_post_for_par_aux (#st:st)
-  (pre_s post_s:st.hprop) (m0 m1:st.mem)
-  (#a:Type) (#pre_f:st.hprop) (#post_f:post_t st a) (lpost_f:l_post pre_f post_f)
-: Lemma
-  (requires
-    preserves_frame pre_s post_s m0 m1 /\
-    st.interp ((pre_s `st.star` pre_f) `st.star` st.locks_invariant m0) m0)
-  (ensures
-    inst_heap_prop_for_par lpost_f m0 (st.core m0) <==>
-    inst_heap_prop_for_par lpost_f m0 (st.core m1))
-= ()
+let frame_post_for_par_aux
+      (#st:st)
+      (pre_s post_s:st.hprop) (m0 m1:st.mem)
+      (#a:Type) (#pre_f:st.hprop) (#post_f:post_t st a) (lpost_f:l_post pre_f post_f)
+    : Lemma
+      (requires
+        preserves_frame pre_s post_s m0 m1 /\
+        st.interp ((pre_s `st.star` pre_f) `st.star` st.locks_invariant m0) m0)
+      (ensures
+        inst_heap_prop_for_par lpost_f m0 (st.core m0) <==>
+        inst_heap_prop_for_par lpost_f m0 (st.core m1))
+    =
+  ()
 
-let frame_post_for_par (#st:st)
-  (pre_s post_s:st.hprop) (m0 m1:st.mem)
-  (#a:Type) (#pre_f:st.hprop) (#post_f:post_t st a) (lpre_f:l_pre pre_f) (lpost_f:l_post pre_f post_f)
-: Lemma
-  (requires
-    preserves_frame pre_s post_s m0 m1 /\
-    st.interp ((pre_s `st.star` pre_f) `st.star` st.locks_invariant m0) m0)
-  (ensures
-    (lpre_f (st.core m0) <==> lpre_f (st.core m1)) /\
-    (forall (x:a) (final_state:st.mem).
-       lpost_f (st.core m0) x final_state <==>
-       lpost_f (st.core m1) x final_state))
-= frame_post_for_par_tautology lpost_f m0;
+let frame_post_for_par
+      (#st:st)
+      (pre_s post_s:st.hprop)
+      (m0 m1:st.mem)
+      (#a:Type)
+      (#pre_f:st.hprop)
+      (#post_f:post_t st a)
+      (lpre_f:l_pre pre_f)
+      (lpost_f:l_post pre_f post_f)
+    : Lemma
+      (requires
+        preserves_frame pre_s post_s m0 m1 /\
+        st.interp ((pre_s `st.star` pre_f) `st.star` st.locks_invariant m0) m0)
+      (ensures
+        (lpre_f (st.core m0) <==> lpre_f (st.core m1)) /\
+        (forall (x:a) (final_state:st.mem).
+          lpost_f (st.core m0) x final_state <==>
+          lpost_f (st.core m1) x final_state))
+    =
+  frame_post_for_par_tautology lpost_f m0;
   frame_post_for_par_aux pre_s post_s m0 m1 lpost_f
-
 
 /// Finally lemmas for proving that in the par rules preconditions get weaker
 ///   and postconditions get stronger
 
-let par_weaker_lpre_and_stronger_lpost_l (#st:st) (#preL:st.hprop) (lpreL:l_pre preL)
-  (#aL:Type) (#postL:post_t st aL) (lpostL:l_post preL postL)
-  (#next_preL:st.hprop) (#next_postL:post_t st aL) (next_lpreL:l_pre next_preL) (next_lpostL:l_post next_preL next_postL)
-  (#preR:st.hprop) (lpreR:l_pre preR)
-  (#aR:Type) (#postR:post_t st aR) (lpostR:l_post preR postR)
-  (state next_state:st.mem)
-: Lemma
-  (requires
-    weaker_lpre lpreL next_lpreL state next_state /\
-    stronger_lpost lpostL next_lpostL state next_state /\
-    preserves_frame preL next_preL state next_state /\
-    lpreL (st.core state) /\
-    lpreR (st.core state) /\
-    st.interp ((preL `st.star` preR) `st.star` st.locks_invariant state) state)
-  (ensures
-    weaker_lpre
-      (par_lpre lpreL lpreR)
-      (par_lpre next_lpreL lpreR)
-      state next_state /\
-    stronger_lpost
-      (par_lpost lpreL lpostL lpreR lpostR)
-      (par_lpost next_lpreL next_lpostL lpreR lpostR)
-      state next_state)
-= frame_post_for_par preL next_preL state next_state lpreR lpostR;
+let par_weaker_lpre_and_stronger_lpost_l
+      (#st:st)
+      (#preL:st.hprop)
+      (lpreL:l_pre preL)
+      (#aL:Type)
+      (#postL:post_t st aL)
+      (lpostL:l_post preL postL)
+      (#next_preL:st.hprop)
+      (#next_postL:post_t st aL)
+      (next_lpreL:l_pre next_preL)
+      (next_lpostL:l_post next_preL next_postL)
+      (#preR:st.hprop)
+      (lpreR:l_pre preR)
+      (#aR:Type)
+      (#postR:post_t st aR)
+      (lpostR:l_post preR postR)
+      (state next_state:st.mem)
+    : Lemma
+      (requires
+        weaker_lpre lpreL next_lpreL state next_state /\
+        stronger_lpost lpostL next_lpostL state next_state /\
+        preserves_frame preL next_preL state next_state /\
+        lpreL (st.core state) /\
+        lpreR (st.core state) /\
+        st.interp ((preL `st.star` preR) `st.star` st.locks_invariant state) state)
+      (ensures
+        weaker_lpre
+          (par_lpre lpreL lpreR)
+          (par_lpre next_lpreL lpreR)
+          state next_state /\
+        stronger_lpost
+          (par_lpost lpreL lpostL lpreR lpostR)
+          (par_lpost next_lpreL next_lpostL lpreR lpostR)
+          state next_state)
+    =
+  frame_post_for_par preL next_preL state next_state lpreR lpostR;
   assert (weaker_lpre (par_lpre lpreL lpreR) (par_lpre next_lpreL lpreR) state next_state) by
     (norm [delta_only [`%weaker_lpre; `%par_lpre] ])
 
-let par_weaker_lpre_and_stronger_lpost_r (#st:st) (#preL:st.hprop) (lpreL:l_pre preL)
-  (#aL:Type) (#postL:post_t st aL) (lpostL:l_post preL postL)
-  (#preR:st.hprop) (lpreR:l_pre preR)
-  (#aR:Type) (#postR:post_t st aR) (lpostR:l_post preR postR)
-  (#next_preR:st.hprop) (#next_postR:post_t st aR) (next_lpreR:l_pre next_preR)
-  (next_lpostR:l_post next_preR next_postR)
-  (state next_state:st.mem)
-: Lemma
-  (requires
-    weaker_lpre lpreR next_lpreR state next_state /\
-    stronger_lpost lpostR next_lpostR state next_state /\
-    preserves_frame preR next_preR state next_state /\
-    lpreR (st.core state) /\
-    lpreL (st.core state) /\
-    st.interp ((preL `st.star` preR) `st.star` st.locks_invariant state) state)
-  (ensures
-    st.interp ((preL `st.star` next_preR) `st.star` st.locks_invariant next_state) next_state /\
-    weaker_lpre
-      (par_lpre lpreL lpreR)
-      (par_lpre lpreL next_lpreR)
-      state next_state /\
-    stronger_lpost
-      (par_lpost lpreL lpostL lpreR lpostR)
-      (par_lpost lpreL lpostL next_lpreR next_lpostR)
-      state next_state)
-= commute_star_right (st.locks_invariant state) preL preR;
+let par_weaker_lpre_and_stronger_lpost_r
+      (#st:st)
+      (#preL:st.hprop)
+      (lpreL:l_pre preL)
+      (#aL:Type)
+      (#postL:post_t st aL)
+      (lpostL:l_post preL postL)
+      (#preR:st.hprop)
+      (lpreR:l_pre preR)
+      (#aR:Type)
+      (#postR:post_t st aR)
+      (lpostR:l_post preR postR)
+      (#next_preR:st.hprop)
+      (#next_postR:post_t st aR)
+      (next_lpreR:l_pre next_preR)
+      (next_lpostR:l_post next_preR next_postR)
+      (state next_state:st.mem)
+    : Lemma
+      (requires
+        weaker_lpre lpreR next_lpreR state next_state /\
+        stronger_lpost lpostR next_lpostR state next_state /\
+        preserves_frame preR next_preR state next_state /\
+        lpreR (st.core state) /\
+        lpreL (st.core state) /\
+        st.interp ((preL `st.star` preR) `st.star` st.locks_invariant state) state)
+      (ensures
+        st.interp ((preL `st.star` next_preR) `st.star` st.locks_invariant next_state) next_state /\
+        weaker_lpre
+          (par_lpre lpreL lpreR)
+          (par_lpre lpreL next_lpreR)
+          state next_state /\
+        stronger_lpost
+          (par_lpost lpreL lpostL lpreR lpostR)
+          (par_lpost lpreL lpostL next_lpreR next_lpostR)
+        state next_state)
+    =
+  commute_star_right (st.locks_invariant state) preL preR;
   apply_interp_ext
     (st.locks_invariant state `st.star` (preL `st.star` preR))
     (st.locks_invariant state `st.star` (preR `st.star` preL))
@@ -873,66 +1031,85 @@ let par_weaker_lpre_and_stronger_lpost_r (#st:st) (#preL:st.hprop) (lpreL:l_pre 
     next_state
 
 #push-options "--warn_error -271"
-let stronger_post_par_r (#st:st) (#aL #aR:Type u#a)
-  (postL:post_t st aL) (postR:post_t st aR) (next_postR:post_t st aR)
-: Lemma
-  (requires stronger_post postR next_postR)
-  (ensures
-    forall xL xR frame h.
-      st.interp ((postL xL `st.star` next_postR xR) `st.star` frame) h ==>
-      st.interp ((postL xL `st.star` postR xR) `st.star` frame) h)
-= let aux xL xR frame h
+let stronger_post_par_r
+      (#st:st)
+      (#aL #aR:Type u#a)
+      (postL:post_t st aL)
+      (postR:post_t st aR)
+      (next_postR:post_t st aR)
     : Lemma
-      (requires st.interp ((postL xL `st.star` next_postR xR) `st.star` frame) h)
-      (ensures st.interp ((postL xL `st.star` postR xR) `st.star` frame) h)
-      [SMTPat ()]
-    = calc (st.equals) {
-        (postL xL `st.star` next_postR xR) `st.star` frame;
-           (st.equals) { }
-        (next_postR xR `st.star` postL xL) `st.star` frame;
-           (st.equals) { }
-        next_postR xR `st.star` (postL xL `st.star` frame);
-      };
-
-      assert (st.interp (next_postR xR `st.star` (postL xL `st.star` frame)) h);
-
-      assert (st.interp (postR xR `st.star` (postL xL `st.star` frame)) h);
-
-      calc (st.equals) {
-        postR xR `st.star` (postL xL `st.star` frame);
-           (st.equals) { }
-        (postR xR `st.star` postL xL) `st.star` frame;
-           (st.equals) { }
-        (postL xL `st.star` postR xR) `st.star` frame;
-      } in
+      (requires stronger_post postR next_postR)
+      (ensures
+        forall xL xR frame h.
+          st.interp ((postL xL `st.star` next_postR xR) `st.star` frame) h ==>
+          st.interp ((postL xL `st.star` postR xR) `st.star` frame) h)
+    =
+  let aux xL xR frame h
+      : Lemma
+        (requires st.interp ((postL xL `st.star` next_postR xR) `st.star` frame) h)
+        (ensures st.interp ((postL xL `st.star` postR xR) `st.star` frame) h)
+        [SMTPat ()]
+      =
+    calc (st.equals) {
+      (postL xL `st.star` next_postR xR) `st.star` frame;
+         (st.equals) { }
+      (next_postR xR `st.star` postL xL) `st.star` frame;
+         (st.equals) { }
+      next_postR xR `st.star` (postL xL `st.star` frame);
+    };
+    assert (st.interp (next_postR xR `st.star` (postL xL `st.star` frame)) h);
+    assert (st.interp (postR xR `st.star` (postL xL `st.star` frame)) h);
+    calc (st.equals) {
+      postR xR `st.star` (postL xL `st.star` frame);
+         (st.equals) { }
+      (postR xR `st.star` postL xL) `st.star` frame;
+         (st.equals) { }
+      (postL xL `st.star` postR xR) `st.star` frame;
+    }
+  in
   ()
 #pop-options
 
 
 (**** Begin stepping functions ****)
 
-let step_ret (#st:st) (#a:Type u#a)
-  (#pre:st.hprop) (#post:post_t st a) (#lpre:l_pre pre) (#lpost:l_post pre post)
-  (f:m st a pre post lpre lpost{Ret? f})
-
-: Mst (step_result st a) (step_req f) (step_ens f)
-
-= NMSTATE?.reflect (fun (_, n) ->
+let step_ret
+      (#st:st)
+      (#a:Type u#a)
+      (#pre:st.hprop)
+      (#post:post_t st a)
+      (#lpre:l_pre pre)
+      (#lpost:l_post pre post)
+      (f:m st a pre post lpre lpost{Ret? f})
+    : Mst (step_result st a) (step_req f) (step_ens f)
+    =
+  NMSTATE?.reflect (fun (_, n) ->
     let Ret p x lp = f in
     Step (p x) p lpre lpost f, n)
 
-let lpost_ret_act (#st:st) (#a:Type) (#pre:st.hprop) (#post:post_t st a) (lpost:l_post pre post)
-  (x:a) (state:st.mem)
-: l_post (post x) post
-= fun _ x h1 -> lpost (st.core state) x h1
+let lpost_ret_act
+      (#st:st)
+      (#a:Type)
+      (#pre:st.hprop)
+      (#post:post_t st a)
+      (lpost:l_post pre post)
+      (x:a)
+      (state:st.mem)
+    : l_post (post x) post
+    =
+  fun _ x h1 -> lpost (st.core state) x h1
 
-let step_act (#st:st) (#a:Type u#a)
-  (#pre:st.hprop) (#post:post_t st a) (#lpre:l_pre pre) (#lpost:l_post pre post)
-  (f:m st a pre post lpre lpost{Act? f})
-
-: Mst (step_result st a) (step_req f) (step_ens f)
-
-= let m0 = get () in
+let step_act
+      (#st:st)
+      (#a:Type u#a)
+      (#pre:st.hprop)
+      (#post:post_t st a)
+      (#lpre:l_pre pre)
+      (#lpost:l_post pre post)
+      (f:m st a pre post lpre lpost{Act? f})
+    : Mst (step_result st a) (step_req f) (step_ens f)
+    =
+  let m0 = get () in
 
   let Act #_ #_ #_ #_ #_ #_ f = f in
 
@@ -942,39 +1119,49 @@ let step_act (#st:st) (#a:Type u#a)
 
   Step (post x) post (fun h -> lpost h x h) lpost (Ret post x lpost)
 
-
 module M = MST
 
-
-let step_bind_ret_aux (#st:st)
-  (#a:Type) (#pre:st.hprop) (#post:post_t st a) (#lpre:l_pre pre) (#lpost:l_post pre post)
-  (f:m st a pre post lpre lpost{Bind? f /\ Ret? (Bind?.f f)})
-
-: M.MSTATE (step_result st a) st.mem st.locks_preorder (step_req f) (step_ens f)
-
-= M.MSTATE?.reflect (fun m0 ->
+let step_bind_ret_aux
+      (#st:st)
+      (#a:Type)
+      (#pre:st.hprop)
+      (#post:post_t st a)
+      (#lpre:l_pre pre)
+      (#lpost:l_post pre post)
+      (f:m st a pre post lpre lpost{Bind? f /\ Ret? (Bind?.f f)})
+    : M.MSTATE (step_result st a) st.mem st.locks_preorder (step_req f) (step_ens f)
+    =
+  M.MSTATE?.reflect (fun m0 ->
     match f with
     | Bind #_ #_ #_ #_ #_ #_ #_ #post_b #lpre_b #lpost_b (Ret p x _) g ->
       Step (p x) post_b (lpre_b x) (lpost_b x) (g x), m0)
 
-let step_bind_ret (#st:st)
-  (#a:Type) (#pre:st.hprop) (#post:post_t st a) (#lpre:l_pre pre) (#lpost:l_post pre post)
-  (f:m st a pre post lpre lpost{Bind? f /\ Ret? (Bind?.f f)})
-
-: Mst (step_result st a) (step_req f) (step_ens f)
-
-= NMSTATE?.reflect (fun (_, n) -> step_bind_ret_aux f, n)
+let step_bind_ret
+      (#st:st)
+      (#a:Type)
+      (#pre:st.hprop)
+      (#post:post_t st a)
+      (#lpre:l_pre pre)
+      (#lpost:l_post pre post)
+      (f:m st a pre post lpre lpost{Bind? f /\ Ret? (Bind?.f f)})
+    : Mst (step_result st a) (step_req f) (step_ens f)
+    =
+  NMSTATE?.reflect (fun (_, n) -> step_bind_ret_aux f, n)
 
 
 #push-options "--z3rlimit 40"
-let step_bind (#st:st)
-  (#a:Type) (#pre:st.hprop) (#post:post_t st a) (#lpre:l_pre pre) (#lpost:l_post pre post)
-  (f:m st a pre post lpre lpost{Bind? f})
-  (step:step_t)
-
-: Mst (step_result st a) (step_req f) (step_ens f)
-
-= match f with
+let step_bind
+      (#st:st)
+      (#a:Type)
+      (#pre:st.hprop)
+      (#post:post_t st a)
+      (#lpre:l_pre pre)
+      (#lpost:l_post pre post)
+      (f:m st a pre post lpre lpost{Bind? f})
+      (step:step_t)
+    : Mst (step_result st a) (step_req f) (step_ens f)
+    =
+  match f with
   | Bind (Ret _ _ _) _ -> step_bind_ret f
 
   | Bind #_ #b #_ #post_a #_ #_ #_ #post_b #lpre_b #lpost_b f g ->
@@ -1005,13 +1192,17 @@ let step_bind (#st:st)
       (Bind f g)
 #pop-options
 
-let step_frame_ret_aux (#st:st)
-  (#a:Type) (#pre:st.hprop) (#p:post_t st a) (#lpre:l_pre pre) (#lpost:l_post pre p)
-  (f:m st a pre p lpre lpost{Frame? f /\ Ret? (Frame?.f f)})
-
-: M.MSTATE (step_result st a) st.mem st.locks_preorder (step_req f) (step_ens f)
-
-= M.MSTATE?.reflect (fun m0 ->
+let step_frame_ret_aux
+      (#st:st)
+      (#a:Type)
+      (#pre:st.hprop)
+      (#p:post_t st a)
+      (#lpre:l_pre pre)
+      (#lpost:l_post pre p)
+      (f:m st a pre p lpre lpost{Frame? f /\ Ret? (Frame?.f f)})
+    : M.MSTATE (step_result st a) st.mem st.locks_preorder (step_req f) (step_ens f)
+    =
+  M.MSTATE?.reflect (fun m0 ->
     match f with
     | Frame (Ret p x lp) frame f_frame ->
       Step (p x `st.star` frame) (fun x -> p x `st.star` frame)
@@ -1019,23 +1210,30 @@ let step_frame_ret_aux (#st:st)
         lpost
         (Ret (fun x -> p x `st.star` frame) x lpost), m0)
 
-let step_frame_ret (#st:st)
-  (#a:Type) (#pre:st.hprop) (#p:post_t st a) (#lpre:l_pre pre) (#lpost:l_post pre p)
-  (f:m st a pre p lpre lpost{Frame? f /\ Ret? (Frame?.f f)})
+let step_frame_ret
+      (#st:st)
+      (#a:Type)
+      (#pre:st.hprop)
+      (#p:post_t st a)
+      (#lpre:l_pre pre)
+      (#lpost:l_post pre p)
+      (f:m st a pre p lpre lpost{Frame? f /\ Ret? (Frame?.f f)})
+    : Mst (step_result st a) (step_req f) (step_ens f)
+    =
+  NMSTATE?.reflect (fun (_, n) -> step_frame_ret_aux f, n)
 
-: Mst (step_result st a) (step_req f) (step_ens f)
-
-= NMSTATE?.reflect (fun (_, n) -> step_frame_ret_aux f, n)
-
-
-let step_frame (#st:st)
-  (#a:Type) (#pre:st.hprop) (#p:post_t st a) (#lpre:l_pre pre) (#lpost:l_post pre p)
-  (f:m st a pre p lpre lpost{Frame? f})
-  (step:step_t)
-
-: Mst (step_result st a) (step_req f) (step_ens f)
-
-= match f with
+let step_frame
+      (#st:st)
+      (#a:Type)
+      (#pre:st.hprop)
+      (#p:post_t st a)
+      (#lpre:l_pre pre)
+      (#lpost:l_post pre p)
+      (f:m st a pre p lpre lpost{Frame? f})
+      (step:step_t)
+    : Mst (step_result st a) (step_req f) (step_ens f)
+    =
+  match f with
   | Frame (Ret p x lp) frame f_frame -> step_frame_ret f
 
   | Frame #_ #_ #f_pre #_ #_ #_ f frame f_frame ->
@@ -1055,42 +1253,55 @@ let step_frame (#st:st)
       (frame_lpost next_flpre next_flpost f_frame)
       (Frame f frame f_frame)
 
+let step_par_ret_aux
+      (#st:st)
+      (#a:Type)
+      (#pre:st.hprop)
+      (#post:post_t st a)
+      (#lpre:l_pre pre)
+      (#lpost:l_post pre post)
+      (f:m st a pre post lpre lpost{Par? f /\ Ret? (Par?.mL f) /\ Ret? (Par?.mR f)})
+    : M.MSTATE (step_result st a) st.mem st.locks_preorder (step_req f) (step_ens f)
+    =
+  M.MSTATE?.reflect (fun m0 ->
+    match f with
+    | Par #_ #aL #_ #_ #_ #_ (Ret pL xL lpL) #aR #_ #_ #_ #_ (Ret pR xR lpR) ->
+      let lpost : l_post
+        #st #(aL & aR)
+        (pL xL `st.star` pR xR)
+        (fun (xL, xR) -> pL xL `st.star` pR xR)
+      =
+        fun h0 (xL, xR) h1 -> lpL h0 xL h1 /\ lpR h0 xR h1
+      in
+      Step (pL xL `st.star` pR xR) (fun (xL, xR) -> pL xL `st.star` pR xR)
+        (fun h -> lpL h xL h /\ lpR h xR h)
+        lpost
+        (Ret (fun (xL, xR) -> pL xL `st.star` pR xR) (xL, xR) lpost), m0)
 
-let step_par_ret_aux (#st:st)
-  (#a:Type) (#pre:st.hprop) (#post:post_t st a) (#lpre:l_pre pre) (#lpost:l_post pre post)
-  (f:m st a pre post lpre lpost{Par? f /\ Ret? (Par?.mL f) /\ Ret? (Par?.mR f)})
+let step_par_ret
+      (#st:st)
+      (#a:Type)
+      (#pre:st.hprop)
+      (#post:post_t st a)
+      (#lpre:l_pre pre)
+      (#lpost:l_post pre post)
+      (f:m st a pre post lpre lpost{Par? f /\ Ret? (Par?.mL f) /\ Ret? (Par?.mR f)})
+    : Mst (step_result st a) (step_req f) (step_ens f)
+    =
+  NMSTATE?.reflect (fun (_, n) -> step_par_ret_aux f, n)
 
-: M.MSTATE (step_result st a) st.mem st.locks_preorder (step_req f) (step_ens f)
-
-= M.MSTATE?.reflect (fun m0 ->
+let step_par
+      (#st:st)
+      (#a:Type)
+      (#pre:st.hprop)
+      (#post:post_t st a)
+      (#lpre:l_pre pre)
+      (#lpost:l_post pre post)
+      (f:m st a pre post lpre lpost{Par? f})
+      (step:step_t)
+    : Mst (step_result st a) (step_req f) (step_ens f)
+    =
   match f with
-  | Par #_ #aL #_ #_ #_ #_ (Ret pL xL lpL) #aR #_ #_ #_ #_ (Ret pR xR lpR) ->
-
-    let lpost : l_post #st #(aL & aR) (pL xL `st.star` pR xR) (fun (xL, xR) -> pL xL `st.star` pR xR)
-      = fun h0 (xL, xR) h1 -> lpL h0 xL h1 /\ lpR h0 xR h1 in
-
-    Step (pL xL `st.star` pR xR) (fun (xL, xR) -> pL xL `st.star` pR xR)
-      (fun h -> lpL h xL h /\ lpR h xR h)
-      lpost
-      (Ret (fun (xL, xR) -> pL xL `st.star` pR xR) (xL, xR) lpost), m0)
-
-
-let step_par_ret (#st:st)
-  (#a:Type) (#pre:st.hprop) (#post:post_t st a) (#lpre:l_pre pre) (#lpost:l_post pre post)
-  (f:m st a pre post lpre lpost{Par? f /\ Ret? (Par?.mL f) /\ Ret? (Par?.mR f)})
-
-: Mst (step_result st a) (step_req f) (step_ens f)
-
-= NMSTATE?.reflect (fun (_, n) -> step_par_ret_aux f, n)
-
-let step_par (#st:st)
-  (#a:Type) (#pre:st.hprop) (#post:post_t st a) (#lpre:l_pre pre) (#lpost:l_post pre post)
-  (f:m st a pre post lpre lpost{Par? f})
-  (step:step_t)
-
-: Mst (step_result st a) (step_req f) (step_ens f)
-
-= match f with
   | Par (Ret _ _ _) (Ret _ _ _) -> step_par_ret f
 
   | Par #_ #aL #preL #postL #lpreL #lpostL mL #aR #preR #postR #lpreR #lpostR mR ->
@@ -1136,26 +1347,36 @@ let step_par (#st:st)
         (Par mL mR)
     end
 
-let step_weaken (#st:st) (#a:Type u#a)
-  (#pre:st.hprop) (#post:post_t st a) (#lpre:l_pre pre) (#lpost:l_post pre post)
-  (f:m st a pre post lpre lpost{Weaken? f})
-
-: Mst (step_result st a) (step_req f) (step_ens f)
-
-= NMSTATE?.reflect (fun (_, n) ->
+let step_weaken
+      (#st:st)
+      (#a:Type u#a)
+      (#pre:st.hprop)
+      (#post:post_t st a)
+      (#lpre:l_pre pre)
+      (#lpost:l_post pre post)
+      (f:m st a pre post lpre lpost{Weaken? f})
+    : Mst (step_result st a) (step_req f) (step_ens f)
+    =
+  NMSTATE?.reflect (fun (_, n) ->
     let Weaken #_ #_ #pre #post #lpre #lpost #_ #_ #_ #_ #_ f = f in
 
     Step pre post lpre lpost f, n)
 
 /// Step function
 
-let rec step (#st:st) (#a:Type u#a)
-  (#pre:st.hprop) (#post:post_t st a) (#lpre:l_pre pre) (#lpost:l_post pre post)
-  (f:m st a pre post lpre lpost)
-: Mst (step_result st a)
-  (step_req f)
-  (step_ens f)
-= match f with
+let rec step
+      (#st:st)
+      (#a:Type u#a)
+      (#pre:st.hprop)
+      (#post:post_t st a)
+      (#lpre:l_pre pre)
+      (#lpost:l_post pre post)
+      (f:m st a pre post lpre lpost)
+    : Mst (step_result st a)
+      (step_req f)
+      (step_ens f)
+    =
+  match f with
   | Ret _ _ _ -> step_ret f
   | Bind _ _ -> step_bind f step
   | Act _ -> step_act f
@@ -1163,19 +1384,24 @@ let rec step (#st:st) (#a:Type u#a)
   | Par _ _ -> step_par f step
   | Weaken _ _ _ _ -> step_weaken f
 
-
-let rec run (#st:st) (#a:Type u#a) (#pre:st.hprop) (#post:post_t st a)
-  (#lpre:l_pre pre) (#lpost:l_post pre post)
-  (f:m st a pre post lpre lpost)
-: Mst a
-  (requires fun m0 ->
-    st.interp (pre `st.star` st.locks_invariant m0) m0 /\
-    lpre (st.core m0))
-  (ensures fun m0 x m1 ->
-    st.interp (post x `st.star` st.locks_invariant m1) m1 /\
-    lpost (st.core m0) x (st.core m1) /\
-    preserves_frame pre (post x) m0 m1)
-= match f with
+let rec run
+      (#st:st)
+      (#a:Type u#a)
+      (#pre:st.hprop)
+      (#post:post_t st a)
+      (#lpre:l_pre pre)
+      (#lpost:l_post pre post)
+      (f:m st a pre post lpre lpost)
+    : Mst a
+      (requires fun m0 ->
+        st.interp (pre `st.star` st.locks_invariant m0) m0 /\
+        lpre (st.core m0))
+      (ensures fun m0 x m1 ->
+        st.interp (post x `st.star` st.locks_invariant m1) m1 /\
+        lpost (st.core m0) x (st.core m1) /\
+        preserves_frame pre (post x) m0 m1)
+    =
+  match f with
   | Ret _ x _ -> x
 
   | _ ->
@@ -1188,38 +1414,3 @@ let rec run (#st:st) (#a:Type u#a) (#pre:st.hprop) (#post:post_t st a)
     preserves_frame_trans pre new_pre (new_post x) m0 m1 m2;
     preserves_frame_stronger_post pre post new_post x m0 m2;
     x
-
-
-// // // // // (**** Trying to define the layered effect ****)
-
-// // // // // type repr (a:Type) (st:st) (pre:st.hprop) (post:post st a) (lpre:l_pre pre) (lpost:l_post pre post)
-// // // // // = unit -> m st a pre post lpre lpost
-
-
-// // // // // /// This will not be allowed currently as the extra binders must appear before x in the implementation, can change
-
-// // // // // let return (a:Type) (st:st) (post:post st a) (lpost:(x:a -> l_post (post x) post)) (x:a)
-// // // // // : repr a st (post x) post (fun h -> (lpost x) h x h) (lpost x)
-// // // // // = fun _ -> Ret post x (lpost x)
-
-// // // // // let bind (a:Type) (b:Type) (st:st)
-// // // // //   (pre_f:st.hprop) (post_f:post st a) (lpre_f:l_pre pre_f) (lpost_f:l_post pre_f post_f)
-// // // // //   (post_g:post st b) (lpre_g:(x:a -> l_pre (post_f x))) (lpost_g:(x:a -> l_post (post_f x) post_g))
-// // // // //   (f:repr a st pre_f post_f lpre_f lpost_f)
-// // // // //   (g:(x:a -> repr b st (post_f x) post_g (lpre_g x) (lpost_g x)))
-// // // // // : repr b st pre_f post_g
-// // // // //     (bind_lpre lpre_f lpost_f lpre_g)
-// // // // //     (bind_lpost lpre_f lpost_f lpost_g)
-// // // // // = fun _ -> Bind (f ()) (fun x -> g x ())
-
-// // // // // let subcomp (a:Type) (st:st)
-// // // // //   (pre:st.hprop) (post:post st a)
-// // // // //   (lpre_f:l_pre pre) (lpost_f:l_post pre post)
-// // // // //   (lpre_g:l_pre pre) (lpost_g:l_post pre post)
-// // // // //   (f:repr a st pre post lpre_f lpost_f)
-// // // // // : Pure (repr a st pre post lpre_g lpost_g)
-// // // // //   (requires
-// // // // //     (forall h. lpre_g h ==> lpre_f h) /\
-// // // // //     (forall h0 x h1. lpost_f h0 x h1 ==> lpost_g h0 x h1))
-// // // // //   (ensures fun _ -> True)
-// // // // // = fun _ -> Weaken #_ #a #pre #post #lpre_f #lpost_f #lpre_g #lpost_g #() (f ())
